identity.v
@@ -1,0 +1,37 @@
+(** Example of function: the identity *)
+Require Import compiler free_variables krivine lterm.
+
+Definition l_id: lterm := Lambda (Var O)
+.
+
+Definition krivine_id : krivine_code := Grab (Access 0 Nop)
+.
+
+
+(** Identity is closed *)
+Lemma closed_id:
+  closed l_id.
+Proof.
+  unfold closed.
+  unfold l_id.
+  simpl.
+  auto with arith.
+Save.
+
+(** Compilation *)
+Lemma compile_id:
+  comp l_id = krivine_id.
+Proof.
+  unfold l_id.
+  unfold krivine_id.
+  trivial.
+Save.
+
+(** Reverse compilation *)
+Lemma tau_id:
+  tau_code krivine_id = Some l_id.
+Proof.
+  unfold l_id.
+  unfold krivine_id.
+  trivial.
+Save.
